coqsrc/Explicit/MTypeRulesExamples.v
@@ -1,19 +1,27 @@
 Require Import Utf8.
 Require Import Common.MBinder.
 Require Import Explicit.MSyntax.
+Require Import Explicit.ExplicitKind.
 Require Import Explicit.MTypeRules.
 Require Import Coq.Strings.Ascii.
 
+Definition Empty_function {X : Type} (e : Empty_set) : X :=
+  match e with end.
+
+Notation "∅∅" := (Empty_function).
+
 Example Empty_world : world :=
 {|
-  w_effect_t := Empty_set;
-  w_eff_op_t := Empty_function;
-  w_eff_ar   := Empty_function;
-  w_base_t := Empty_set ;
-  w_base_v := Empty_function
+  w_effect_t := ∅;
+  w_eff_op_t := ∅∅;
+  w_eff_ar   := ∅∅;
+  w_base_t   := ∅;
+  w_base_v   := ∅∅
 |}.
 
-Example ew_var {TV:Set} (n:TV) : typ Empty_world TV := t_var n.
+Notation "W∅" := Empty_world.
+
+Example ew_var {TV:Set} (n:TV) : typ W∅ TV := t_var n.
 
 Example row_equivalence_example : 
   〈ew_var 1; ew_var 2; ew_var 3; ew_var 4; ew_var 5〉 ≅ 
@@ -35,17 +43,24 @@ Proof.
   apply row_append_base.
 Qed.
 
-Inductive Example_effect : Set :=
-| IO_effect : Example_effect.
-
-Example IO_effect_operation : Set := inc (inc Empty_set).
-
-Example getc : IO_effect_operation := VZ. 
-Example putc : IO_effect_operation := VS VZ.
+Example guards_operation_example :
+  guards_operation (inc (inc (inc ∅))) (inc (inc ∅)) (VS (VZ)).
+Proof.
+  apply gop_step.
+  apply gop_base.
+Qed.
 
 Inductive Example_base_type : Set :=
 | bt_unit : Example_base_type
 | bt_char : Example_base_type.
+
+Inductive Example_effect : Set :=
+| IO_effect : Example_effect.
+
+Example IO_effect_operation : Set := inc (inc ∅).
+
+Example getc : IO_effect_operation := VZ. 
+Example putc : IO_effect_operation := VS VZ.
 
 Example Example_world : world :=
 {|
@@ -56,58 +71,102 @@ Example Example_world : world :=
   w_base_v   := λ b, match b with | bt_unit => True | bt_char => ascii end
 |}.
 
-Example Example_program := expr Example_world Empty_set Empty_set.
-Example Example_typ := typ Example_world Empty_set.
+Notation EW := Example_world.
+Example Example_typ := typ EW ∅.
+Example Example_program := expr EW ∅ ∅.
 
-Example print_H : Example_program.
+(*Coercion t_base : EW.(w_base_t) >-> Example_typ.*)
+
+Definition Example_operation_types : Operation_types EW.
 Proof.
-  apply e_app.
-  { apply e_value.
-    apply v_eff_op with IO_effect.
-    apply putc. }
-  { apply e_value.
-    apply v_const with bt_char.
-    apply "H"%char. }
+  intros TV. simpl.
+  intros [] _ op.
+  destruct op eqn:op_eqn.
+  + apply (t_base (bt_unit:w_base_t EW), t_base (bt_char:w_base_t EW)).
+  + apply (t_base (bt_char:w_base_t EW), t_base (bt_unit:w_base_t EW)).
 Defined.
 
-Example IO_0_stream_Handler (e : Example_program) : Example_program.
+Example getc_type : ∀ TV eff,
+  Example_operation_types TV eff nil getc = (t_base (bt_unit:w_base_t EW), t_base (bt_char:w_base_t EW)).
 Proof.
-  apply e_handle with IO_effect.
-  { apply nil. }
-  { apply e. }
-  { apply h_op.
-    { apply e_app.
-      { apply e_value.
-        apply v_var.
-        apply V2_resume. }
-      apply e_value.
-      apply v_const with bt_unit.
+  intros.
+  destruct eff.
+  reflexivity.
+Qed.
+
+Example print_H : Example_program :=
+  e_app
+    (v_eff_op (IO_effect:w_effect_t EW) putc)
+    (v_const  (bt_char  :w_base_t   EW) "H"%char).
+
+Example IO_zero_handler : handler EW ∅ ∅ IO_effect_operation :=
+   h_op _ (e_app (v_var V2_resume) (v_const (bt_unit:w_base_t EW) I))
+  (h_op _ (e_app (v_var V2_resume) (v_const (bt_char:w_base_t EW) "000"%char))
+  (h_return (v_var VZ)
+  )).
+
+Example IO_zero_handler_type : ∀ σ_r,
+  σ_r ::[ ∅∅ ] k_type →
+  handler_has_type Example_operation_types ∅∅ ∅∅
+  IO_effect_operation IO_zero_handler IO_effect σ_r σ_r 〈〉.
+Proof.
+  intros σ_r H.
+  apply (HT_op _ _ _ _ (putc:w_eff_op_t EW IO_effect) nil).
+  { apply gop_step.
+    apply gop_base. }
+  { simpl.
+    apply T_App with (t_base (bt_unit:w_base_t EW)).
+    { apply H. }
+    { apply t_base_kind. }
+    { constructor. }
+    { simpl.
+      apply T_Var.
+      { reflexivity. }
       constructor. }
-    apply h_op.
-    { apply e_app.
-      { apply e_value.
-        apply v_var.
-        apply V2_resume. }
-      apply e_value.
-      apply v_const with bt_char.
-      apply "000"%char. }
-    apply h_return.
-    { apply e_value.
-      apply v_var.
-      apply VZ. } }
-Defined.
+    { apply T_Con; constructor. } }
+  apply (HT_op _ _ _ _ (getc:w_eff_op_t EW IO_effect) nil).
+  { apply gop_base. }
+  { simpl.
+    apply T_App with (t_base (bt_char:w_base_t EW)).
+    { apply H. }
+    { apply t_base_kind. }
+    { constructor. }
+    { simpl.
+      apply T_Var.
+      { reflexivity. }
+      constructor. }
+    { apply T_Con; constructor. } }
+  apply HT_return.
+  constructor.
+  + reflexivity.
+  + constructor.
+Qed.
 
-Example Example_bt (b : Example_base_type) : Example_typ.
-Proof.
-  apply t_base.
-  apply b.
-Defined.
+Example handle_example : expr EW ∅ ∅ :=
+  e_handle (IO_effect:w_effect_t EW) nil
+    (e_app
+      (v_eff_op (IO_effect:w_effect_t EW) getc)
+      (v_const (bt_unit:w_base_t EW) I))
+    IO_zero_handler.
 
-Example IO_effect_row : Example_typ.
+Example handle_type_example :
+  (Example_operation_types,(∅∅:∅ → typ EW ∅),(∅∅:∅ → kind)) ⊢
+    handle_example ∈ t_base (bt_char:w_base_t EW) | 〈〉.
 Proof.
-  apply t_row_cons.
-  { apply t_effect.
-    + apply IO_effect.
-    + apply nil. }
-  apply 〈〉.
-Defined.
+  apply T_Handle with (t_base (bt_char:w_base_t EW)).
+  { reflexivity. }
+  { apply IO_zero_handler_type.
+    apply t_base_kind. }
+  apply T_App with (t_base (bt_unit:w_base_t EW)).
+  { apply t_base_kind. }
+  { apply t_base_kind. }
+  { constructor.
+    { apply t_effect_kind.
+      reflexivity. }
+    apply empty_effect_kind. }
+  { apply T_Op with nil.
+    reflexivity. }
+  { apply T_Con.
+    + reflexivity.
+    + repeat(constructor). }
+Qed.
